Alpha structural recursion/induction (#3)
Recursion/Induction combinator

theories/NameAbstraction.v
@@ -1,5 +1,6 @@
 From Coq Require Import Classes.RelationClasses.
-From Nominal Require Import Alpha Instances.Name Instances.Prod.
+From Nominal Require Import Alpha.
+From Nominal.Instances Require Import Name Prod Perm.
 
 #[universes(template=no)]
 Record NameAbstraction `{Nominal X} := mkAbstraction { abs :> (Name * X) }.
@@ -8,24 +9,24 @@ Arguments mkAbstraction {_ _ _ _ _} _.
 Notation " '[𝔸]' X " := (NameAbstraction X) (at level 1, no associativity, format "[𝔸] X").
 Notation " [ a ] x " := ({| abs := (a,x) |}) (at level 1, no associativity, format "[ a ] x").
 
+#[export] Instance name_abstraction_action `{Nominal X}: PermAction [𝔸]X := 
+    λ p a, mkAbstraction (p • (fst a), p • (snd a)). 
+
+#[export] Instance name_abstraction_support `{Nominal X}: Support [𝔸]X := 
+    fun ax => let (a,x) := abs ax in (support x) ∖ {[a]}.
+    
 (* Given X nominal, the pair (name * X) is a nominal type module (≈α) *)
 #[export] Instance name_abstraction_equiv `{Nominal X}: Equiv [𝔸]X := (≈α).
 #[export] Instance name_abstraction_equivalence `{Nominal X}: Equivalence (name_abstraction_equiv (X := X)).
 Proof.
     split; unfold name_abstraction_equiv; repeat intro.
-    - destruct x as [[a x]]; simpl; new b fresh a x; exists b; split; intuition.
+    - destruct x as [[a x]]; simpl; new b fresh a x; fresh_tac; exists b; split; intuition.
     - destruct x as [[a x]]; destruct y as [[b y]]; simpl in *; destruct H1 as [c []];
         exists c; split; intuition.
     - destruct x as [[a x]]; destruct y as [[b y]]; destruct z as [[c z]]; apply alpha_some_any in H1,H2;
-        simpl in *; new f fresh a b c x y z; exists f; split; [intuition | etransitivity]; 
+        simpl in *; new f fresh a b c x y z; fresh_tac; exists f; split; [intuition | etransitivity]; 
         [eapply H1 | eapply H2]; intuition.
 Qed.
-
-#[export] Instance name_abstraction_action `{Nominal X}: PermAction [𝔸]X := 
-    λ p a, mkAbstraction (p • (fst a), p • (snd a)). 
-
-(* FIXME: Por aonde? *)
-#[export] Instance perm_support: Support Perm := λ p, perm_dom p.
 
 #[export] Instance name_abstraction_perm `{Nominal X}: PermT [𝔸]X.
 Proof.
@@ -36,29 +37,45 @@ Proof.
         unfold action, name_abstraction_action, equiv, name_abstraction_equiv.
         unfold equiv, name_abstraction_equiv in Heq2; simpl in *.
         new w fresh p q a b x y (p • x) (q • y); exists w; apply alpha_some_any in Heq2; split.
-        + split_and!; try apply name_fresh_action; auto.
+        + split_and!; try apply name_fresh_action; split_union; apply support_fresh; auto.
         + cut ((p • w ≡ w) ∧ (q • w ≡ w)); [intros [W1 W2] | split; apply perm_notin_domain_id; auto].
             (* slow *)rewrite <-W1 at 1; (* slow *)rewrite <-W2 at 2.
             rewrite 2!gact_compat, <-2!perm_comm_distr, <-2!gact_compat, Heq1.
-            apply perm_inj. unfold alpha_equiv_a in *; apply Heq2; intuition.
+            apply perm_inj. unfold alpha_equiv_a in *; apply Heq2; split_and!; split_union;
+            apply support_fresh; auto. split_union. split_union.
     - intros [[a x]]; unfold action, name_abstraction_action, prod_action, equiv, name_abstraction_equiv; simpl.
         apply alpha_some_any; intros w ?; rewrite 2!gact_id; reflexivity.
     - intros ? ? [[a x]]; unfold action, name_abstraction_action, prod_action, equiv, name_abstraction_equiv;
         apply alpha_some_any; intros w ?; simpl in *; rewrite <-2!gact_compat; reflexivity.
 Qed.
 
-#[export] Instance name_abstraction_support `{Nominal X}: Support [𝔸]X := 
-    λ a, support (abs a).
-
 #[export] Instance name_abstraction_nominal `{Nominal X}: Nominal [𝔸]X.
 Proof. split.
     - exact name_abstraction_perm.
     - intros [[a x]] b c ? ?; destruct (decide (b = c)), (decide (b = a)), (decide (c = a));
           try (subst; congruence || subst; apply perm_action_equal); unfold support, name_abstraction_support in *; simpl in *.
-        + apply support_fresh,fresh_prod_iff in H1 as [?%name_neq_fresh_iff ?]; congruence.
-        + apply support_fresh,fresh_prod_iff in H2 as [?%name_neq_fresh_iff ?]; congruence.
-        + new z fresh (⟨b,c⟩ • a) a (⟨b,c⟩ • x) x; exists z; simpl; split; simpl; [intuition |].
-          rewrite perm_swap_neither, (fresh_fixpoint b c x); auto; apply fresh_prod_iff in H1,H2; intuition.
+        + subst; apply not_elem_of_difference in H1 as []; apply not_elem_of_difference in H2 as [].   (* subst. apply support_fresh in H1. as [?%name_neq_fresh_iff ?]. congruence. *)
+          * unfold action,equiv,name_abstraction_equiv,name_abstraction_action ; simpl.
+            rewrite name_action_left. pose proof (@Equivalence_Symmetric _ _ alpha_equivalence_e) as S.
+            symmetry; apply alpha_rename, support_fresh; auto.
+          * set_solver.
+          * unfold action,equiv,name_abstraction_equiv,name_abstraction_action ; simpl.
+            rewrite name_action_left. pose proof (@Equivalence_Symmetric _ _ alpha_equivalence_e) as S.
+            symmetry; apply alpha_rename, support_fresh; auto.
+          * set_solver.  
+        + subst; apply not_elem_of_difference in H1 as []; apply not_elem_of_difference in H2 as [].
+          * unfold action,equiv,name_abstraction_equiv,name_abstraction_action ; simpl.
+            rewrite name_action_right; pose proof (@Equivalence_Symmetric _ _ alpha_equivalence_e) as S.
+            symmetry. apply alpha_rename_swap, support_fresh; auto.
+          * unfold action,equiv,name_abstraction_equiv,name_abstraction_action ; simpl.
+            rewrite name_action_right; pose proof (@Equivalence_Symmetric _ _ alpha_equivalence_e) as S.
+            symmetry; apply alpha_rename_swap, support_fresh; auto.
+          * set_solver.
+          * set_solver. 
+        + new z fresh (⟨b,c⟩ • a) a (⟨b,c⟩ • x) x; fresh_tac; exists z; simpl; split; simpl; [intuition |].
+          rewrite perm_swap_neither, (fresh_fixpoint b c x); auto.
+          * apply not_elem_of_difference in H1 as []; apply support_fresh; auto; set_solver.
+          * apply not_elem_of_difference in H2 as []; apply support_fresh; auto; set_solver.
 Qed.
 
 (* Basic properties *)
@@ -66,10 +83,14 @@ Lemma name_abstraction_rename `{Nominal X} (a b: Name) (x: X):
     b#x → [a]x ≡ [b](⟨a,b⟩ • x).
 Proof. apply alpha_rename. Qed.
 
+Lemma name_abstraction_rename_swap `{Nominal X} (a b: Name) (x: X): 
+    b#x → [a]x ≡ [b](⟨b,a⟩ • x).
+Proof. apply alpha_rename_swap. Qed.
+
 Lemma nabs_action `{Nominal X} p a (x: X): p • [a]x = [p • a](p • x).
 Proof. auto. Qed.
 
-Lemma nabs_support `{Nominal X} a (x: X): support [a]x = support a ∪ support x.
+Lemma nabs_support `{Nominal X} a (x: X): support [a]x = support x ∖ {[a]}.
 Proof. auto. Qed.
 
 Lemma nabs_inv `{Nominal X} a (x x': X): [a]x ≡ [a]x' ↔ x ≡ x'.
@@ -80,17 +101,19 @@ Qed.
 
 Lemma fresh_same_alpha_class `{Nominal X} a (x: X): a # [a]x.
 Proof.
-    destruct (exist_fresh (support a ∪ support x)) as [w ?]; exists w.
+    destruct (exist_fresh (support x ∖ {[a]})) as [w ?]; exists w.
     split; [auto |].
-    unfold equiv, name_abstraction_equiv; simpl.
-    rewrite perm_swap_left; apply alpha_inv_iff; right; split.
-    - apply fresh_prod_iff; split; apply support_fresh; set_solver.
-    - rewrite swap_perm; reflexivity.
+    apply not_elem_of_difference in H1 as [].
+    + unfold equiv, name_abstraction_equiv; simpl.
+      rewrite name_action_left; pose proof (@Equivalence_Symmetric _ _ alpha_equivalence_e) as S;
+      symmetry; apply alpha_rename, support_fresh; assumption.
+    + apply elem_of_singleton in H1; subst; apply perm_action_equal.
 Qed.
 
-Lemma alpha_class_inv1 `{Nominal X} (a a': Name) (x: X): a = a' ∨ a' # x → a' # [a]x.
+Lemma alpha_class_inv1 `{Nominal X} (a a': Name) (x: X): 
+    a = a' ∨ (a ≠ a' ∧ a' # x) → a' # [a]x.
 Proof.
-    intros [EqA | F]; [rewrite EqA | destruct (decide (a = a')); subst]; try apply fresh_same_alpha_class.
+    intros [EqA | [? F]]; [rewrite EqA | destruct (decide (a = a')); subst]; try apply fresh_same_alpha_class.
     destruct (exist_fresh (support a ∪ support a' ∪ support x)) as [w ?]; exists w.
     split; [set_solver |].
     unfold equiv, name_abstraction_equiv; simpl.
@@ -98,10 +121,11 @@ Proof.
     apply alpha_inv_name_equiv_iff, fresh_fixpoint; [assumption | apply support_fresh]; set_solver.
 Qed.
 
-Lemma alpha_class_inv2 `{Nominal X} (a a': Name) (x: X): a' # [a]x → a = a' ∨ a' # x.
+Lemma alpha_class_inv2 `{Nominal X} (a a': Name) (x: X): 
+    a' # [a]x → a = a' ∨ (a ≠ a' ∧ a' # x).
 Proof.
     intros F; destruct (decide (a = a')); subst; [intuition |].
-    right. (* a ≠ a' *)
+    right. (* a ≠ a' *) split; auto.
     destruct (exist_fresh (support a ∪ support a' ∪ support x ∪ support [a]x)) as [w ?]; exists w.
     split; [set_solver |]; apply some_any_iff in F; cut (w ∉ support [a]x); [intros Hw | set_solver].
     specialize (F w Hw); unfold equiv, name_abstraction_equiv in F. 
@@ -109,5 +133,78 @@ Proof.
     rewrite L in F; apply alpha_inv_name_equiv_iff in F; assumption.
 Qed.
 
-Lemma alpha_class_inv `{Nominal X} (a a': Name) (x: X): a = a' ∨ a' # x ↔ a' # [a]x.
+Lemma alpha_class_inv `{Nominal X} (a a': Name) (x: X): 
+    a = a' ∨ (a ≠ a' ∧ a' # x) ↔ a' # [a]x.
 Proof. split; [apply alpha_class_inv1 | apply alpha_class_inv2]. Qed.
+
+#[global] Instance name_abstraction_rw1 `{Nominal X}: 
+    ∀a, Proper (equiv ==> alpha_equiv_e) (pair a).
+Proof. repeat intro; apply alpha_inv_iff; left; tauto. Qed.
+
+#[global] Instance name_abstraction_rw2 `{Nominal X}: 
+    Proper (alpha_equiv_e ==> (@name_abstraction_equiv X _ _ _ _)) mkAbstraction.
+Proof. repeat intro; unfold name_abstraction_equiv; simpl; assumption. Qed.
+
+#[global] Instance name_abstraction_rw3 `{Nominal X}: 
+    Proper ((@name_abstraction_equiv X _ _ _ _) ==> (@name_abstraction_equiv X _ _ _ _) ==> flip impl) equiv.
+Proof.
+    repeat intro; unfold name_abstraction_equiv in *; 
+    destruct x as [[a x]]; destruct y as [[a' x']];
+    destruct x0 as [[b z]]; destruct y0 as [[b' z']]; simpl; unfold equiv in *.
+    (* for some reason Coq cant find an instance for Transitive or Symmetric alpha_equiv_e *)
+    pose proof (@Equivalence_Transitive _ _ alpha_equivalence_e) as T.
+    pose proof (@Equivalence_Symmetric _ _ alpha_equivalence_e) as S.
+    apply T with [a']x'; auto; apply T with [b']z'; auto.
+Qed.
+
+#[global] Instance name_abstraction_rw4 `{Nominal X}: 
+    ∀ a (x : X), ProperProxy ((@name_abstraction_equiv X _ _ _ _)) [a]x.
+Proof. 
+    unfold ProperProxy,name_abstraction_equiv; repeat intro.
+    pose proof (@Equivalence_Reflexive _ _ alpha_equivalence_e) as F.
+    auto.
+Qed.
+
+Lemma name_abstraction_inv `{Nominal} (a b: Name) (x y: X):
+    [a]x ≡ [b]y ↔ (a = b ∧ x ≡ y) ∨ ((a # [b]y) ∧ x ≡ ⟨a,b⟩ • y).
+Proof.
+    split; intro HH.
+    - apply alpha_inv_iff in HH as [? | [HHH ?]].
+        + left; assumption.
+        + right; split; try tauto; apply alpha_class_inv; right; apply fresh_prod_iff in HHH as []; split.
+            * apply not_eq_sym, name_neq_fresh_iff; assumption.
+            * assumption. 
+    - destruct HH as [[] | [HH1 HH2]].
+        + subst; rewrite H2; reflexivity.
+        + apply alpha_class_inv in HH1 as []; subst.
+            * apply nabs_inv; rewrite HH2; apply perm_action_equal.
+            * apply alpha_inv_iff; right; split.
+                -- apply fresh_prod_iff; split; [apply name_fresh_iff,name_neq_fresh_iff |]; tauto.
+                -- assumption.
+Qed.
+
+(* Concretion *)
+Section Concretion.
+    Context `{Nominal X}.
+
+    Definition concretion (F: [𝔸]X) (b: Name): option X :=
+       let (a,x) := abs F in
+       if (decide (a = b)) then Some x else
+       if (decide (b ∉ support x)) then Some (⟨a,b⟩ • x)
+       else None.
+    
+    Lemma concretion_eq a b (x: X): 
+        a = b → concretion ([a]x) b ≡ Some x.
+    Proof. 
+        intros; subst; unfold concretion; simpl; destruct (decide _); subst;
+        [reflexivity | congruence].
+    Qed.
+
+    Lemma concretion_notin a b (x: X): 
+        a ≠ b → b ∉ support x → concretion ([a]x) b ≡ Some (⟨a,b⟩ • x).
+    Proof. 
+        intros; subst; unfold concretion; simpl; destruct (decide _); subst;
+        [congruence | destruct (decide _); [reflexivity | set_solver]]. 
+    Qed.
+    
+End Concretion.
