theories/Instances/Name.v
@@ -22,6 +22,9 @@ Proof.
     auto.
 Qed.
 
+Lemma union_empty (A : NameSet) : A ≡ A ∪ ∅.
+Proof. set_solver. Qed.
+
 (* Freshness properties for name *)
 Lemma name_fresh_neq1 (a b: Name): a # b → a ≠ b.
 Proof. 
@@ -39,6 +42,12 @@ Qed.
 Lemma name_neq_fresh_iff (a b: Name): a # b ↔ a ≠ b.
 Proof. split; [apply name_fresh_neq1 | apply name_fresh_neq2]. Qed.
 
+Lemma name_fresh_iff (a b: Name): a # b ↔ b # a.
+Proof. 
+    split; intro H; apply name_neq_fresh_iff in H; apply name_neq_fresh_iff;
+    apply not_eq_sym; assumption.
+Qed.
+
 Lemma name_fresh_action p (a b: Name): b # a → b ∉ perm_dom p → b # (p • a).
 Proof.
     intros HH ?; destruct (exist_fresh (support a ∪ support b ∪ perm_dom p ∪ support (p • a))) as [w ?];
@@ -53,3 +62,15 @@ Proof.
     intros [? [H1 H2]]; unfold support, name_support in *; apply not_elem_of_singleton_1 in H1.
     rewrite perm_swap_left in H2; congruence.
 Qed.
+
+Lemma name_action_left (a b: Name) : ⟨a,b⟩ • a ≡ b.
+Proof. unfold action, name_action; apply perm_swap_left. Qed.
+
+Lemma name_action_right (a b: Name) : ⟨a,b⟩ • b ≡ a.
+Proof. unfold action, name_action; apply perm_swap_right. Qed.
+
+Lemma name_action_neither (a b c: Name) : c ≠ a → c ≠ b → ⟨a,b⟩ • c ≡ c.
+Proof. intros; unfold action, name_action; apply perm_swap_neither; auto. Qed.
+
+Lemma nameset_fresh_respect (A B: NameSet): A ≡ B → fresh A ≡ fresh B.
+Proof. intros AB; rewrite AB; reflexivity. Qed.
