theories/Instances/SupportedFunctions.v
@@ -1,5 +1,20 @@
 From Nominal Require Import Nominal.
 
+(* Normal functions *)
+Section FunGact.
+  Context `{PermT X, PermT Y}.
+
+  #[global] Instance fun_action : PermAction (X → Y) :=
+    λ (p: Perm) (f: X → Y), (λ (x: X), p • f(((-p) • x))).
+
+  #[global] Instance fun_equiv : Equiv (X → Y) := 
+    λ f g, ∀ (x: X), f x ≡@{Y} g x.
+
+  #[global] Instance fun_equiv_equivalence : Equivalence fun_equiv.
+  Proof. split; repeat intro; [reflexivity | symmetry | etransitivity]; eauto. Qed.  
+
+End FunGact.
+
 Section SupportedFunctions.
   Context (X Y: Type) `{Nominal X, Nominal Y}.
 
@@ -17,9 +32,13 @@ Arguments f_supp {_ _ _ _ _ _} _.
 #[export] Existing Instance f_proper.
 
 Notation "'λₛ' x .. y , t" :=
-  (@mkFunSupp _ _ _ _ _ _ (λ x, .. (@mkFunSupp _ _ _ _ _ _ (λ y, t) _ _ _) ..) _ _ _)
+  (@mkFunSupp _ _ _ _ _ _ (fun x => .. (@mkFunSupp _ _ _ _ _ _ (fun y => t) _ _ _) ..) _ _ _)
   (at level 200, x binder, y binder, right associativity).
 
+Notation "'λₛ⟦' S '⟧' x .. y , t" :=
+  (@mkFunSupp _ _ _ _ _ _ (fun x => .. (@mkFunSupp _ _ _ _ _ _ (fun y => t) S _ _) ..) S _ _)
+  (at level 200, x binder, y binder, right associativity).
+  
 Notation " A '→ₛ' B " := (FunSupp A B) (at level 99, B at level 200, right associativity).
 
 Section FunSuppProperties.
@@ -32,8 +51,8 @@ Section FunSuppProperties.
     #[global] Instance fun_supp_proper: Proper (fun_supp_equiv ⟹ (≡@{X}) ⟹ (≡@{Y})) (f_car X Y).
     Proof. intros ? ? HH1 ? ? HH2; rewrite HH2; apply HH1. Qed. 
 
-    #[refine] Instance fun_supp_act: PermAction (X →ₛ Y) :=
-      λ (p: Perm) (f: X →ₛ Y), (λₛ (x: X), p • f((-p) • x)).
+    #[refine,global] Instance fun_supp_act: PermAction (X →ₛ Y) :=
+      λ (p: Perm) (f: X →ₛ Y), (λₛ (x: X), p • ( f(((-p) • (x))) )).
     Proof. 
       all:try (assumption || typeclasses eauto).
       - exact ((f_supp f) ∪ (perm_dom p)).
@@ -65,6 +84,29 @@ Section FunSuppProperties.
         simpl; intros; rewrite <-perm_inv; apply f_supp_spec; assumption.
     Qed.
 End FunSuppProperties.
+
+Lemma fsupp_equiv `{Nominal X, Nominal Y} (f: X →ₛ Y) (x x' : X) : x ≡ x' → f x ≡ f x'.
+Proof. intros XX; rewrite XX; reflexivity. Qed.
+
+Lemma fsupp_equiv2 `{Nominal X, Nominal Y, Nominal Z} (f: X →ₛ (Y →ₛ Z)) (x x' : X) (y y' : Y): 
+  x ≡ x' → y ≡ y' → f x y ≡ f x' y'.
+Proof. intros XX YY; rewrite XX, YY; reflexivity. Qed.
+
+Lemma fsupp_equiv3 `{Nominal X, Nominal Y, Nominal Z, Nominal W}
+ (f: X →ₛ (Y →ₛ (Z →ₛ W))) (x x' : X) (y y' : Y) (z z' : Z): 
+  x ≡ x' → y ≡ y' → z ≡ z' → f x y z ≡ f x' y' z'.
+Proof. intros XX YY ZZ; rewrite XX, YY, ZZ; reflexivity. Qed.
+
+Lemma fsupp_action `{Nominal X, Nominal Y} (p : Perm) (f : X →ₛ Y) (x : X):
+  (p • f)(x) ≡ p • f(-p • x).
+Proof. unfold action at 1; unfold fun_supp_act; simpl; reflexivity. Qed. 
+
+Lemma fun_equivar `{Nominal X, Nominal Y} (p : Perm) (f: X →ₛ Y) (x : X):
+  p • (f x) ≡ (p • f)(p • x).
+Proof.
+  unfold action at 2; unfold fun_supp_act; simpl. 
+  rewrite perm_left_inv; reflexivity.
+Qed.
 
 From Nominal Require Import Fresh.
 
